Added resources for aof; going with hocap style

src/program_proof/lockservice/aof_proof.v
@@ -1,56 +1,73 @@
 From Perennial.program_proof Require Import proof_prelude.
 From Goose.github_com.mit_pdos.gokv Require Import aof.
 From Perennial.goose_lang Require Import ffi.grove_ffi.
+From Perennial.algebra Require Import mlist auth_map.
+From iris.algebra Require Import mono_nat.
 
 Section aof_proof.
 Context `{!heapG Σ}.
 Context `{!filesysG Σ}.
 
-Class aofG Σ := LockserviceG {
-  ls_rpcG :> inG Σ (prodR fracR (exclR (leibnizO (list u8)))) ;
+Class aofG Σ := AofG {
+  aof_flistG :> fmlistG u8 Σ
 }.
 
 Record aof_vol_names := {
   logdata : gname ;
   predurabledata : gname ;
+  len : gname ;
+  len_toks : gname ;
 }.
 
 Context `{!aofG Σ}.
-
-Definition own_flist γ (q:Qp) (l:list u8) :=
-  own γ (q, (Excl (l:leibnizO (list u8)))).
+Context `{!inG Σ mono_natUR}.
+Context `{!mapG Σ u64 unit}.
 
 Implicit Types γ : aof_vol_names.
+Implicit Types aof_ctx : (list u8) → iProp Σ.
 
-Definition aof_mu_invariant (aof_ptr:loc) γ : iProp Σ :=
+Definition aof_len_invariant γ : iProp Σ :=
+  ∃ (l:u64),
+    own γ.(len) (mono_nat_auth (1/2) (int.nat l)) ∗
+    [∗ set] x ∈ (fin_to_set u64), x [[γ.(len_toks)]]↦ () ∨ ⌜int.nat x > int.nat l⌝
+.
+
+Definition aof_mu_invariant (aof_ptr:loc) γ aof_ctx : iProp Σ :=
   ∃ membuf_sl membufC predurableC (durlen:u64),
   "Hmembuf" ∷ aof_ptr ↦[AppendOnlyFile.S :: "membuf"] (slice_val membuf_sl) ∗
   "HdurableLength" ∷ aof_ptr ↦[AppendOnlyFile.S :: "durableLength"]{1/2} #durlen ∗
   "Hmembuf_sl" ∷ typed_slice.is_slice membuf_sl byteT 1 membufC ∗
-  "Hpredurable" ∷ own_flist γ.(predurabledata) (1/2) predurableC ∗
-  "Hlogdata" ∷ own_flist γ.(logdata) (1/2)%Qp (predurableC ++ membufC)
+  "Hpredurable" ∷ fmlist γ.(predurabledata) (1/2) predurableC ∗
+  "Hlogdata" ∷ fmlist γ.(logdata) (1/2)%Qp (predurableC ++ membufC) ∗
+  "Hlen_toks" ∷ ([∗ set] x ∈ (fin_to_set u64), x [[γ.(len_toks)]]↦ () ∨ ⌜int.nat x < length (predurableC ++ membufC)⌝) ∗
+  "Hmembuf_fupd" ∷ (aof_ctx predurableC ={⊤}=∗ aof_ctx (predurableC ++ membufC)
+     ∗ (own γ.(len) (mono_nat_auth (1/2) (length predurableC)) ={⊤}=∗
+        own γ.(len) (mono_nat_auth (1/2) (length (predurableC ++ membufC)))
+       )
+  )
 .
 
 Definition aofN := nroot .@ "aof".
 
-Definition is_aof aof_ptr γ : iProp Σ :=
+Definition is_aof aof_ptr γ (aof_ctx : (list u8) → iProp Σ) : iProp Σ :=
   ∃ mu_ptr (lenCond_ptr durCond_ptr:loc),
   "#Hmu" ∷ readonly (aof_ptr ↦[AppendOnlyFile.S :: "mu"] mu_ptr) ∗
   "#HlengthCond" ∷ readonly (aof_ptr ↦[AppendOnlyFile.S :: "lengthCond"] #lenCond_ptr) ∗
   "#HdurableCond" ∷ readonly (aof_ptr ↦[AppendOnlyFile.S :: "durableCond"] #durCond_ptr) ∗
   "#HlenCond" ∷ is_cond lenCond_ptr mu_ptr ∗
   "#HdurCond" ∷ is_cond durCond_ptr mu_ptr ∗
-  "#Hmu_inv" ∷ is_lock aofN mu_ptr (aof_mu_invariant aof_ptr γ)
+  "#Hmu_inv" ∷ is_lock aofN mu_ptr (aof_mu_invariant aof_ptr γ aof_ctx)
 .
 
 (* TODO: upgrade to WPC *)
-Lemma wp_CreateAppendOnlyFile (fname:string) :
+Lemma wp_CreateAppendOnlyFile (fname:string) data aof_ctx :
   {{{
-       (∃ data, fname f↦{1} data)
+       fname f↦{1} data ∗
+       aof_ctx data
   }}}
     CreateAppendOnlyFile #(str fname)
   {{{
-       aof_ptr γ, RET #aof_ptr; is_aof aof_ptr γ
+       aof_ptr γ, RET #aof_ptr; is_aof aof_ptr γ aof_ctx
   }}}.
 Proof.
   iIntros (Φ) "Hpre HΦ".
@@ -63,7 +80,6 @@ Proof.
   iNamed "Hl".
 
   wp_pures.
-  Search (lock.new).
   wp_apply (wp_new_free_lock).
   iIntros (mu) "Hmu_free".
 
@@ -86,34 +102,30 @@ Proof.
      us filemapsto as part of mu. I think keeping the ctx in the loop would be
      more "hocap" style.
    *)
+  (*
+    Going to go with hocap-style approach: seems easier to not lose any information in membuf_fupd.
+    Otherwise, the membuf_fupd would say "|={Eo,Ei}=> fileptsto old ∗ fileptsto new ={Ei,Eo}=∗ emp",
+    which isn't enough to chain with a new fupd.
+   *)
   admit.
 Admitted.
 
 Definition aof_log_own γ data :=
-  own_flist γ.(logdata) (1/2)%Qp data.
+  fmlist γ.(logdata) (1/2)%Qp data.
 
-Lemma flist_combine (γ:gname) q q' data data' :
-  own_flist γ q data -∗
-  own_flist γ q' data' -∗
-  own_flist γ (q + q') data.
-Proof.
+Definition aof_length_lb γ (l:u64) : iProp Σ.
 Admitted.
 
-Lemma update_flist data' (γ:gname) data:
-  own_flist γ 1 data ==∗
-  own_flist γ 1 data'
-.
-Proof.
-Admitted.
-
-Lemma wp_AppendOnlyFile__Append aof_ptr γ data_sl (oldData newData:list u8) :
-is_aof aof_ptr γ -∗
+Lemma wp_AppendOnlyFile__Append aof_ptr γ data_sl aof_ctx (oldData newData:list u8) Q :
+is_aof aof_ptr γ aof_ctx -∗
   {{{
-       typed_slice.is_slice data_sl byteT 1 newData ∗ aof_log_own γ oldData
+       typed_slice.is_slice data_sl byteT 1 newData ∗ aof_log_own γ oldData ∗
+       (aof_ctx oldData ={⊤}=∗ aof_ctx (oldData ++ newData) ∗ Q)
   }}}
     AppendOnlyFile__Append #aof_ptr (slice_val data_sl)
   {{{
-       (l:u64), RET #l; aof_log_own γ (oldData ++ newData)
+       (l:u64), RET #l; aof_log_own γ (oldData ++ newData) ∗
+                        (aof_length_lb γ l ={⊤}=∗ Q)
   }}}.
 Proof.
   iIntros "#Haof" (Φ) "!# Hpre HΦ".
@@ -125,7 +137,7 @@ Proof.
   wp_apply (acquire_spec with "Hmu_inv").
   iIntros "[Hlocked Haof]".
   iNamed "Haof".
-  iDestruct "Hpre" as "[HnewData Haof_log]".
+  iDestruct "Hpre" as "(HnewData & Haof_log & Hfupd)".
   wp_pures.
 
   wp_loadField.
@@ -147,7 +159,15 @@ Proof.
 
   wp_pures.
 
-  (* TODO: Update logical list *)
+
+  unfold aof_log_own.
+  iDestruct (fmlist_agree_1 with "Haof_log Hlogdata") as %->.
+  iCombine "Haof_log Hlogdata" as "Haof_log".
+
+  iMod (fmlist_update ((predurableC ++ membufC) ++ newData) with "Haof_log") as "[Haof_log _]".
+  { admit. (* have to prove list prefix... don't really care since we want flist, not fmlist *) }
+
+  iDestruct "Haof_log" as "[Hlogdata Haof_log]".
 
   wp_loadField.
   wp_apply (release_spec with "[-HΦ Haof_log]").
@@ -155,13 +175,21 @@ Proof.
     iFrame "#∗".
     iNext.
     iExists _, _, _, _.
+    rewrite -app_assoc.
     iFrame.
-    (* update logical list above *)
-    admit.
+
+    iIntros "Haof_ctx".
+    (* TODO: need to do this before, so we can also deal with the Q *)
+    iMod ("Hmembuf_fupd" with "Haof_ctx") as "Haof_ctx".
+    iMod ("Hfupd" with "Haof_ctx") as "[Haof_ctx HQ]".
+    iModIntro.
+    iFrame.
   }
   wp_pures.
   iApply "HΦ".
-  (* same update as above *)
+  iFrame.
+
+  (* Need to set up mnat, tokens, and some invariants to prove this. *)
 Admitted.
 
 End aof_proof.
